Various updates...
Modifications to misc/total-order.lisp:
 - add fast-lexorder and fast-<< functions,
 - optimize << (via MBE) to use fast-<< as its :exec
 - document << and these new functions with xdoc

Modifications to osets:
 - document osets with xdoc
 - take advantage of fast-lexorder/fast-<< in some definitions
 - other various minor changes

books/finite-set-theory/osets/membership.lisp
@@ -14,25 +14,9 @@
 
 ; membership.lisp
 ;
-; We are now getting into more interesting territory.  The primitive set
-; functions nicely contain the potential messes that we would have to face if
-; we were implementing sets just using the primitive list functions.  However,
-; they are still plagued with order.
-;
-; The end user of the set library should not have to care that the elements of
-; the set are ordered or not.  (Well, with the exception that if they are
-; trying to make a fast version of a function, they might decide to exploit
-; that order.)
-;
-; Set reasoning should be done in terms of membership.  In traditional
-; mathematics, subsets are defined through quantification over membership, as
-; is set equailty, and so forth.  But right now, the best we can do is induct
-; over insert, which is somewhat messy.
-;
 ; This file introduces the notions of set membership and subset.  We also go
-; into an abstract argument which will form the basis for quantification.  The
-; goal is to transform the insertion induction proofs into more traditional
-; pick-a-point and double containment proofs.
+; into an abstract argument which will form the basis for quantification, and
+; especially for pick-a-point and double containment proofs.
 ;
 ; At the end of this file, we will disable all of the theorems that pertain to
 ; the order of elements, providing an entirely membership-based reasoning
@@ -44,104 +28,141 @@
 (set-verify-guards-eagerness 2)
 
 
+(defsection in
+  :parents (osets)
+  :short "@(call in) determines if <tt>a</tt> is a member of the set
+<tt>X</tt>."
 
-; Set Membership.
-;
-; We could go ahead and write another version of in, which could use the total
-; order to stop early if it ever encountered an element too big.  I.e., looking
-; for 1 in the list '(2 3 4), it could say that since 1 << 2, we are done.
-;
-; Should we do so?  Really the only question is whether or not it would be
-; faster.  Certainly we can contrive situations in which it would be better,
-; i.e. (in 1 '(2 3 4 .... 100000)), where we would save 100,000 calls to in.
-; But we can also contrive situations that it would be slower, for example (in
-; 100001 '(1 2 3 4 ... 100000)), where we would incur the extra cost of 100,000
-; calls to <<.
-;
-; I have arbitrarily decided not to implement short-circuiting.  My reasoning
-; is that (1) it is not clear which would be faster, (2) it is not clear what
-; "typical" usage behavior of in would be, so even if we wanted to benchmark
-; the two solutions, we could probably not come up with a good benchmarking
-; suite, (3) both solutions are O(n) anyway so I don't think there's much to be
-; gained here, and (4) the current method is arguably "no less efficient" than
-; an unordered implementation.
+  :long "<p>The logical definition of <tt>in</tt> makes no mention of the set
+order, except implicitly by the use of the set @(see primitives) like @(see
+head) and @(see tail).</p>
 
-(defun in (a X)
-  (declare (xargs :guard (setp X)
-                  :verify-guards nil))
-  (mbe :logic
-       (and (not (empty X))
-            (or (equal a (head X))
-                (in a (tail X))))
-       :exec
+<p>The :exec version just inlines the set primitives and does one level of loop
+unrolling.  On CCL, it seems to run about 2.6x faster on the following
+loop:</p>
 
-; On CCL, the :exec version is almost 3x faster on the following
-; microbenchmark; logic mode: 5.014 seconds, exec mode: 1.732 seconds; inlining
-; without unrolling 2.15 seconds.  Further unrolling doesn't appear to be
-; beneficial.
-;
-; (let ((big-set (loop for i from 1 to 100000 collect i)))
-;   (gc$)
-;   (time (loop for i fixnum from 1 to 30000 do (sets::in i big-set))))
+<code>
+ ;; 4.703 sec logic, 1.811 sec exec
+ (let ((big-set (loop for i from 1 to 100000 collect i)))
+   (gc$)
+   (time (loop for i fixnum from 1 to 30000 do (sets::in i big-set))))
+</code>
 
-       (and x
-            (or (equal a (car x))
-                (and (cdr x)
-                     (or (equal a (cadr x))
-                         (in a (cddr x))))))))
+<p>There are other ways we could optimize <tt>in</tt>.  Since the set is
+ordered, we could try to use the set order @(see <<) to stop early when we ran
+into an element that is larger than the one we are looking for.  For instance,
+when looking for 1 in the set '(2 3 4), we know that since <tt>1 &lt;&lt;
+2</tt> that <tt>1</tt> cannot be a member of this set.</p>
 
-(verify-guards in
-  :hints(("Goal" :in-theory (enable (:ruleset primitive-rules)))))
+<p>The simplest way to do this is to use <tt>&lt;&lt;</tt> at every element.
+But set order comparisons can be very expensive, especially when sets contain
+large cons structures.  So while it is easy to contrive situations where
+exploiting the order would be advantageous, like</p>
 
-(defthm in-type
-  (or (equal (in a X) t)
-      (equal (in a X) nil))
-  :rule-classes :type-prescription)
+<code>
+ (in 1 '(2 3 4 .... 100000))
+</code>
 
-(encapsulate ()
+<p>where we could return instantly, there are also times where it would be
+slower.  For instance, on</p>
 
-  (local (defthm head-not-whole
-           (implies (not (empty X))
-                    (not (equal (head X) X)))
-           :hints(("Goal" :in-theory (enable (:ruleset primitive-rules))))))
+<code>
+ (in 100001 '(1 2 3 4 ... 100000))
+</code>
 
-  (local (defthm lemma
-    (implies (> (acl2-count x) (acl2-count y))
-             (not (in x y)))))
+<p>we would incur the extra cost of 100,000 calls to <tt>&lt;&lt;</tt>.</p>
 
-  (defthm not-in-self
-    (not (in x x))))
+<p>For this reason, we do not currently implement any short-circuiting.  The
+reasoning is:</p>
 
-(defthm in-sfix-cancel
-  (equal (in a (sfix X))
-         (in a X)))
+<ul>
 
-(defthm never-in-empty
-  (implies (empty X)
-           (not (in a X))))
+<li>it is not clear which would be faster in all cases,</li>
 
-(defthm in-set
-  (implies (in a X)
-           (setp X)))
+<li>it is not clear what the typical usage behavior of <tt>in</tt> is, so even
+if we wanted to benchmark alternate implementations, it may be hard to come up
+with the right benchmarking suite</li>
 
-(defthm in-tail
-  (implies (in a (tail X))
+<li>both solutions are O(n) anyway, and <tt>in</tt> isn't a function that
+should probably be used in any kind of loop so its performance shouldn't be
+especially critical to anything</li>
+
+<li>the current method is arguably no less efficient than an unordered
+implementation.</li>
+
+</ul>
+
+<p>Future note.  In principle membership in an ordered list might be done in
+<tt>O(log_2 n)</tt>.  We are considering using a <i>galloping</i> membership
+check in the future to obtain something along these lines.</p>"
+
+  (defun in (a X)
+    (declare (xargs :guard (setp X)
+                    :verify-guards nil))
+    (mbe :logic
+         (and (not (empty X))
+              (or (equal a (head X))
+                  (in a (tail X))))
+         :exec
+         (and x
+              (or (equal a (car x))
+                  (and (cdr x)
+                       (or (equal a (cadr x))
+                           (in a (cddr x))))))))
+
+  (verify-guards in
+    :hints(("Goal" :in-theory (enable (:ruleset primitive-rules)))))
+
+  (defthm in-type
+    (or (equal (in a X) t)
+        (equal (in a X) nil))
+    :rule-classes :type-prescription)
+
+  (encapsulate ()
+
+    (local (defthm head-not-whole
+             (implies (not (empty X))
+                      (not (equal (head X) X)))
+             :hints(("Goal" :in-theory (enable (:ruleset primitive-rules))))))
+
+    (local (defthm lemma
+             (implies (> (acl2-count x) (acl2-count y))
+                      (not (in x y)))))
+
+    (defthm not-in-self
+      (not (in x x))))
+
+  (defthm in-sfix-cancel
+    (equal (in a (sfix X))
            (in a X)))
 
-(defthm in-tail-or-head
-  (implies (and (in a X)
-                (not (in a (tail X))))
-           (equal (head X) a)))
+  (defthm never-in-empty
+    (implies (empty X)
+             (not (in a X))))
 
-(defthm in-head
-  ;; BOZO seems redundant with never-in-empty
-  (equal (in (head X) X)
-         (not (empty X))))
+  (defthm in-set
+    (implies (in a X)
+             (setp X)))
+
+  (defthm in-tail
+    (implies (in a (tail X))
+             (in a X)))
+
+  (defthm in-tail-or-head
+    (implies (and (in a X)
+                  (not (in a (tail X))))
+             (equal (head X) a)))
+
+  (defthm in-head
+    ;; BOZO seems redundant with never-in-empty
+    (equal (in (head X) X)
+           (not (empty X)))))
 
 
 ; We now begin to move away from set order.
 
-(encapsulate ()
+(defsection head-unique
+  :extension head
 
   (local (defthm lemma
 	   (implies (and (not (empty X))
@@ -161,430 +182,540 @@
 
   (defthm head-minimal-2
     (implies (in a X)
-	     (not (<< a (head X))))))
+	     (not (<< a (head X)))))
 
-(add-to-ruleset order-rules '(head-minimal head-minimal-2))
+  (add-to-ruleset order-rules '(head-minimal head-minimal-2))
 
-(encapsulate ()
 
-  (local (defthm lemma
+  (local (defthm lemma2
 	   (implies (empty (tail X))
 		    (not (in (head X) (tail X))))))
 
-  (local (defthm lemma-2
+  (local (defthm lemma3
 	   (implies (not (empty (tail X)))
 		    (not (in (head X) (tail X))))
 	   :hints(("Goal" :in-theory (enable (:ruleset order-rules))))))
 
-  ;; This is an interesting theorem, which gives us a concept of
-  ;; uniqueness without using the set order to state it!
+  ;; This is an interesting theorem, which gives us a concept of uniqueness
+  ;; without using the set order to state it!
 
   (defthm head-unique
     (not (in (head X) (tail X)))
     :hints(("Goal"
-	    :use ((:instance lemma)
-		  (:instance lemma-2))))))
-
-
-(defthm insert-identity
-  (implies (in a X)
-           (equal (insert a X) X))
-  :hints(("Goal" :in-theory (enable (:ruleset order-rules)))))
-
-
-(defthm in-insert
-  (equal (in a (insert b X))
-         (or (in a X)
-             (equal a b)))
-  :hints(("Goal" :in-theory (enable (:ruleset order-rules))
-                 :induct (insert b X))))
+	    :use ((:instance lemma2)
+		  (:instance lemma3))))))
 
 
 
+(defsection in-insert
+  :extension insert
 
-; The behavior of insert is, of course, determined by the set order.  Yet, we
-; often need to induct upon insert's definition to prove theorems.  So, here we
-; introduce a new induction scheme which hides the set order, yet still allows
-; us to induct on insert very nicely.  We then disable the induction scheme
-; that insert normally uses, and set up an induction hint so that
-; weak-insert-induction will automatically be used instead.
+  (defthm insert-identity
+    (implies (in a X)
+             (equal (insert a X) X))
+    :hints(("Goal"
+            :in-theory (enable (:ruleset order-rules)))))
 
-(defthm weak-insert-induction-helper-1
-  (implies (and (not (in a X))
-                (not (equal (head (insert a X)) a)))
-           (equal (head (insert a X))
-                  (head X)))
-  :hints(("Goal" :in-theory (enable (:ruleset order-rules)))))
-
-(defthm weak-insert-induction-helper-2
-  (implies (and (not (in a X))
-                (not (equal (head (insert a X)) a)))
-           (equal (tail (insert a X))
-                  (insert a (tail X))))
-  :hints(("Goal" :in-theory (enable (:ruleset order-rules)))))
-
-(defthm weak-insert-induction-helper-3
-  (implies (and (not (in a X))
-                (equal (head (insert a X)) a))
-           (equal (tail (insert a X))
-                  (sfix X)))
-  :hints(("Goal" :in-theory (enable (:ruleset order-rules)))))
-
-(defun weak-insert-induction (a X)
-  (declare (xargs :guard (setp X)))
-  (cond ((empty X) nil)
-        ((in a X) nil)
-        ((equal (head (insert a X)) a) nil)
-        (t (list (weak-insert-induction a (tail X))))))
-
-(in-theory (disable (:induction insert)))
-
-(defthm use-weak-insert-induction t
-  :rule-classes ((:induction
-                  :pattern (insert a X)
-                  :scheme (weak-insert-induction a X))))
+  (defthm in-insert
+    (equal (in a (insert b X))
+           (or (in a X)
+               (equal a b)))
+    :hints(("Goal"
+            :in-theory (enable (:ruleset order-rules))
+            :induct (insert b X)))))
 
 
 
+(defsection weak-insert-induction
+  :parents (insert)
+  :short "Inducting over insert without exposing the set order."
 
+  :long "<p>When we want to insert an element into an ordered set, the set
+order obviously has to be involved so that we can decide where to put the new
+element.  Accordingly, the set order plays a role in the induction scheme that
+we get from @(see insert)'s definition.  This makes insert somewhat different
+than other set operations (membership, union, cardinality, etc.) that just use
+a simple @(see tail)-based induction, where the set order is already hidden by
+<tt>tail</tt>.</p>
 
-; Subset Testing.
-;
-; Now we introduce subset.  This becomes complicated because we want to use MBE
-; to make it fast.  The fast-subset function is a tail recursive, linear pass
-; through both lists.  Subset, by comparison, is a nice to reason about
-; definition and much simpler, but would require quadratic time if we didn't
-; use MBE here.
+<p>When we are proving theorems about sets, we generally want to avoid thinking
+about the set order, but we sometimes need to induct over <tt>insert</tt>.  So,
+here we introduce a new induction scheme that allows us to induct over insert
+but hides the set order.  We disable the ordinary induction scheme that insert
+uses, and set up an induction hint so that <tt>weak-insert-induction</tt> will
+automatically be used instead.</p>"
 
-(defun fast-subset (X Y)
-  (declare (xargs :guard (and (setp X) (setp Y))
-                  :guard-hints(("Goal" :in-theory (enable (:ruleset primitive-rules) <<)))))
-  (mbe :logic
-       (cond ((empty X) t)
-             ((empty Y) nil)
-             ((<< (head X) (head Y)) nil)
-             ((equal (head X) (head Y)) (fast-subset (tail X) (tail Y)))
-             (t (fast-subset X (tail Y))))
-       :exec
+  (defthm weak-insert-induction-helper-1
+    (implies (and (not (in a X))
+                  (not (equal (head (insert a X)) a)))
+             (equal (head (insert a X))
+                    (head X)))
+    :hints(("Goal" :in-theory (enable (:ruleset order-rules)))))
 
-; Per the following microbenchmark, the :exec version is about 2.3x faster
-; than the logic mode definition; logic mode: 3.74 seconds; exec mode: 1.62
-; seconds
-;
-; (let ((x (loop for i from 1 to 1000 collect i)))
-;   (gc$)
-;   (time$ (loop for i fixnum from 1 to 100000 do (sets::fast-subset x x))))
+  (defthm weak-insert-induction-helper-2
+    (implies (and (not (in a X))
+                  (not (equal (head (insert a X)) a)))
+             (equal (tail (insert a X))
+                    (insert a (tail X))))
+    :hints(("Goal" :in-theory (enable (:ruleset order-rules)))))
 
-       (cond ((null X) t)
-             ((null Y) nil)
-             ((lexorder (car X) (car Y))
-              (and (equal (car X) (car Y))
-                   (fast-subset (cdr X) (cdr Y))))
-             (t
-              (fast-subset X (cdr Y))))))
+  (defthm weak-insert-induction-helper-3
+    (implies (and (not (in a X))
+                  (equal (head (insert a X)) a))
+             (equal (tail (insert a X))
+                    (sfix X)))
+    :hints(("Goal" :in-theory (enable (:ruleset order-rules)))))
 
-(defun subset (X Y)
-  (declare (xargs :guard (and (setp X) (setp Y))
-                  :verify-guards nil))
-  (mbe :logic (if (empty X)
-		  t
-		(and (in (head X) Y)
-		     (subset (tail X) Y)))
-       :exec (fast-subset X Y)))
+  (defun weak-insert-induction (a X)
+    (declare (xargs :guard (setp X)))
+    (cond ((empty X) nil)
+          ((in a X) nil)
+          ((equal (head (insert a X)) a) nil)
+          (t (list (weak-insert-induction a (tail X))))))
 
-(defthm subset-type
-  (or (equal (subset X Y) t)
-      (equal (subset X Y) nil))
-  :rule-classes :type-prescription)
+  (in-theory (disable (:induction insert)))
 
-(encapsulate ()
-
-  (local (defthmd lemma
-	   (implies (not (in (head Y) X))
-		    (equal (subset X Y)
-                           (subset X (tail Y))))))
-
-  (local (defthm case-1
-	   (implies (and (not (empty X))
-			 (not (empty Y))
-			 (not (<< (head X) (head Y)))
-			 (not (equal (head X) (head Y)))
-			 (implies (and (setp X) (setp (tail Y)))
-				  (equal (fast-subset X (tail Y))
-					 (subset X (tail Y)))))
-		    (implies (and (setp X) (setp Y))
-			     (equal (fast-subset X Y)
-				    (subset X Y))))
-	   :hints(("Goal" :in-theory (enable (:ruleset order-rules))
-		   :use (:instance lemma)))))
-
-  (local (defthm case-2
-	   (implies (and (not (empty x))
-			 (not (empty y))
-			 (not (<< (head x) (head y)))
-			 (equal (head x) (head y))
-			 (implies (and (setp (tail x)) (setp (tail y)))
-				  (equal (fast-subset (tail x) (tail y))
-					 (subset (tail x) (tail y)))))
-		    (implies (and (setp x) (setp y))
-			     (equal (fast-subset x y)
-				    (subset x y))))
-	   :hints(("Goal" :in-theory (enable (:ruleset order-rules))
-		   :use (:instance lemma (X (tail X)))))))
-
-  (local (defthm fast-subset-equivalence
-	   (implies (and (setp X) (setp Y))
-		    (equal (fast-subset X Y)
-                           (subset X Y)))
-	   :hints(("Goal" :in-theory (enable (:ruleset order-rules))
-		   :induct (fast-subset X Y)))))
-
-  (verify-guards subset))
+  (defthm use-weak-insert-induction t
+    :rule-classes ((:induction
+                    :pattern (insert a X)
+                    :scheme (weak-insert-induction a X)))))
 
 
 
+(defsection subset
+  :parents (osets)
+  :short "@(call subset) determines if <tt>X</tt> is a subset of <tt>Y</tt>."
 
-; Quantification over Sets.
-; BOZO we should probably switch to the witness-cp stuff.
-;
-; Up until version 0.81, we used an explicit argument to reduce subset proofs
-; to pick-a-point style membership arguments.  Starting in 0.9, we generalize
-; this argument to arbitrary predicates instead.
-;
-; I'll begin with some background on what we historically wanted to do.  The
-; "ultimate goal" was to use pick-a-point reasoning to prove subset
-; relationships.  In traditional mathematics, subset is defined using
-; quantification over members, e.g., as follows:
-;
-;    (subset X Y) iff "forall a : (in a X) implies (in a Y)"
-;
-; Traditionally, one would prove the membership part of this statement, and use
-; it to conclude whether or not (subset X Y) is true.  But, in ACL2, we cannot
-; write a theorem of the following form, because all variables are implicitly
-; universally quantified.
-;
-;    [ "forall a : (in a ...) implies (in a ___)" ]
-;       =>
-;    (subset ... ___)
-;
-; However, we can take the contrapositive of this theorem, which looks like the
-; following:
-;
-;    ~(subset ... ___) => "exists a : (in a ...) ^ ~(in a ___)
-;
-; And we can prove this, by using a new function to search for an element which
-; satisfies the existential predicate.
-;
-; Once we prove the above, we still need to be able to "reduce" a proof of
-; (subset X Y) to a proof of (in a X) => (in a Y).  While we can't do this with
-; a direct rewrite rule, we can sort of fake it using functional instantiation.
-; In other words, we set up an encapsulated event with (in a X) => (in a Y) as
-; its constraint, then we can use this constraint to prove that (subset X Y).
-; By functionally instantiating the resulting theorem, we can reduce the subset
-; problem to a membership problem.
-;
-; All of this was an explicit argument until version 0.9.  But, now the process
-; is generalized.  First notice that subset is really nothing more than "forall
-; a, (in a x) => (in a Y)."  If you let (P x) = (in a Y), then this is "forall
-; a, (in a x) => (P a)".  This is a more general concept which can capture not
-; only subset, but also many other ideas by simply changing the meaning of (P
-; x).  For example, if P = integerp, then we can test if every element in the
-; set is an integer, and so forth.  So, starting in v0.9, we use this more
-; general form of encapsulate instead of the more specific version used in
-; previous versions.
-;
-; We begin by introducing a completely arbitrary predicate.  Based on this
-; generic predicate we will introduce a new function, all, which checks to see
-; if every member in a set satisfies a predicate.  We also introduce find-not,
-; which can be used to find us a witness for proving all-by-membership.
-; Finally, we set up an encapsulate which allows us to assume that if some
-; hypotheses are true, then any member of some set satisfies the predicate, and
-; use this constraint to prove that if those same hypotheses are satisfied,
-; then all is true for the same set.
+  :long "<p>We use a logically simple definition, but using MBE we exploit the
+set order to implement a tail-recursive, linear subset check.</p>
 
-(encapsulate
- (((predicate *) => *))
-  (local (defun predicate (x) x)))
+<p>The :exec version of fast-subset just inlines the set primitives and tweaks
+the way the order check is done.  It is about 3x faster than the :logic version
+of fast-subset on the following loop:</p>
 
-(defun all (set-for-all-reduction)
-  (declare (xargs :guard (setp set-for-all-reduction)))
-  (if (empty set-for-all-reduction)
-      t
-    (and (predicate (head set-for-all-reduction))
-	 (all (tail set-for-all-reduction)))))
+<code>
+ ;; 3.83 sec logic, 1.24 seconds exec
+ (let ((x (loop for i from 1 to 1000 collect i)))
+   (gc$)
+   (time$ (loop for i fixnum from 1 to 100000 do (sets::subset x x))))
+</code>
 
-(defun find-not (X)
-  (declare (xargs :guard (setp X)))
-  (cond ((empty X) nil)
-	((not (predicate (head X))) (head X))
-	(t (find-not (tail X)))))
+<p>In the future we may investigate developing a faster subset check based on
+galloping.</p>"
+
+  (defun fast-subset (X Y)
+    (declare (xargs :guard (and (setp X) (setp Y))
+                    :guard-hints(("Goal" :in-theory (enable (:ruleset primitive-rules) <<)))))
+    (mbe :logic
+         (cond ((empty X) t)
+               ((empty Y) nil)
+               ((<< (head X) (head Y)) nil)
+               ((equal (head X) (head Y)) (fast-subset (tail X) (tail Y)))
+               (t (fast-subset X (tail Y))))
+         :exec
+         (cond ((null X) t)
+               ((null Y) nil)
+               ((fast-lexorder (car X) (car Y))
+                (and (equal (car X) (car Y))
+                     (fast-subset (cdr X) (cdr Y))))
+               (t
+                (fast-subset X (cdr Y))))))
+
+  (defun subset (X Y)
+    (declare (xargs :guard (and (setp X) (setp Y))
+                    :verify-guards nil))
+    (mbe :logic
+         (if (empty X)
+                    t
+                  (and (in (head X) Y)
+                       (subset (tail X) Y)))
+         :exec (fast-subset X Y)))
+
+  (defthm subset-type
+    (or (equal (subset X Y) t)
+        (equal (subset X Y) nil))
+    :rule-classes :type-prescription)
+
+  (encapsulate ()
+
+    (local (defthmd lemma
+             (implies (not (in (head Y) X))
+                      (equal (subset X Y)
+                             (subset X (tail Y))))))
+
+    (local (defthm case-1
+             (implies (and (not (empty X))
+                           (not (empty Y))
+                           (not (<< (head X) (head Y)))
+                           (not (equal (head X) (head Y)))
+                           (implies (and (setp X) (setp (tail Y)))
+                                    (equal (fast-subset X (tail Y))
+                                           (subset X (tail Y)))))
+                      (implies (and (setp X) (setp Y))
+                               (equal (fast-subset X Y)
+                                      (subset X Y))))
+             :hints(("Goal" :in-theory (enable (:ruleset order-rules))
+                     :use (:instance lemma)))))
+
+    (local (defthm case-2
+             (implies (and (not (empty x))
+                           (not (empty y))
+                           (not (<< (head x) (head y)))
+                           (equal (head x) (head y))
+                           (implies (and (setp (tail x)) (setp (tail y)))
+                                    (equal (fast-subset (tail x) (tail y))
+                                           (subset (tail x) (tail y)))))
+                      (implies (and (setp x) (setp y))
+                               (equal (fast-subset x y)
+                                      (subset x y))))
+             :hints(("Goal" :in-theory (enable (:ruleset order-rules))
+                     :use (:instance lemma (X (tail X)))))))
+
+    (local (defthm fast-subset-equivalence
+             (implies (and (setp X) (setp Y))
+                      (equal (fast-subset X Y)
+                             (subset X Y)))
+             :hints(("Goal" :in-theory (enable (:ruleset order-rules))
+                     :induct (fast-subset X Y)))))
+
+    (verify-guards subset)))
 
 
 
-(encapsulate
- (((all-hyps) => *)
-  ((all-set) => *))
+(defsection all-by-membership
+  :parents (osets)
+  :short "A way to quantify over sets."
 
- (local (defun all-hyps () nil))
- (local (defun all-set () nil))
+  :long "<p><tt>all-by-membership</tt> is a generic theorem that can be used to
+prove that a property holds of a set by showing that a related property holds
+of the set elements.</p>
 
- (defthmd membership-constraint
-   (implies (all-hyps)
-	    (implies (in arbitrary-element (all-set))
-		     (predicate arbitrary-element)))))
+<p>The most important role of <tt>all-by-membership</tt> is to allow for
+pick-a-point proofs of @(see subset).  That is, it allows us to show that
+<tt>(subset X Y)</tt> holds by showing that every element of X satisfies
+<tt>(in a Y)</tt>.</p>
 
-(encapsulate ()
+<p>More generally, we could show that a set satisfies a predicate like
+<tt>integer-setp</tt> because each of its elements satisfies
+<tt>integerp</tt>.</p>
+
+
+<h3>Pick-a-Point Proofs in ACL2</h3>
+
+<p>We begin by explaining how pick-a-point proofs of subset can be carried out.
+In traditional mathematics, @(see subset) is defined using quantification over
+members, e.g., as follows:</p>
+
+<code>
+  (equal (subset X Y)
+         (forall a (implies (in a X) (in a Y))))
+</code>
+
+<p>This definition is very useful for <b>pick-a-point</b> proofs that some set
+<tt>X</tt> is a subset of <tt>Y</tt>.  Such a proof begins by picking an
+arbitrary point <tt>a</tt> that is a member of <tt>X</tt>.  Then, if we can
+show that <tt>a</tt> must be a member of <tt>Y</tt>, we have established
+<tt>(subset X Y)</tt>.</p>
+
+<p>These kinds of arguments are extremely useful, and we would like to be able
+to carry them out in ACL2 about osets.  But since ACL2 does not have explicit
+quantifiers, we cannot even write a theorem like this:</p>
+
+<code>
+ (implies (forall a (implies (in a X) (in a Y)))
+          (subset X Y))
+</code>
+
+<p>But consider the contrapositive of this theorem:</p>
+
+<code>
+ (implies (not (subset X Y))
+          (exists a (and (in a X) (not (in a Y)))))
+</code>
+
+<p>We <i>can</i> prove something like this, by writing an explicit function to
+search for an element of <tt>X</tt> that is not an element of <tt>Y</tt>.  That
+is, we can prove:</p>
+
+<code>
+ (implies (not (subset X Y))
+          (let ((a (find-witness X Y)))
+            (and (in a X)
+                 (not (in a Y)))))
+</code>
+
+<p>Once we prove the above, we still need to be able to \"reduce\" a proof of
+<tt>(subset X Y)</tt> to a proof of <tt>(implies (in a X) (in a Y))</tt>.
+While we can't do this with a direct rewrite rule, we can sort of fake it using
+functional instantiation.  As groundwork:</p>
+
+<ul>
+
+<li>Using @(see encapsulate), we introduce functions <tt>sub</tt> and
+<tt>super</tt> with the constraint that
+<code>
+ (implies (in a (sub))
+          (in a (super)))
+</code></li>
+
+<li>Using this constraint, we prove the generic theorem:
+<code>
+ (subset (sub) (super))
+</code></li>
+
+</ul>
+
+<p>Then, when we want to prove <tt>(subset X Y)</tt> for some particular
+<tt>X</tt> and <tt>Y</tt>, we can functionally instantiate the generic theorem
+with</p>
+
+<code>
+   sub   &lt;-- (lambda () X)
+   super &lt;-- (lambda () Y)
+</code>
+
+<p>And this allows us to prove <tt>(subset X Y)</tt> as long as we can relieve
+the constraint, i.e., <tt>(implies (in a X) (in a Y))</tt>.</p>
+
+
+<h3>Generalizing Pick-a-Point Proofs</h3>
+
+<p>In earlier versions of the osets library, we used an explicit argument to
+reduce subset proofs to pick-a-point style membership arguments.  But we later
+generalized the approach to arbitrary predicates instead.</p>
+
+<p>First, notice that if you let the predicate <tt>(P a)</tt> be defined as
+<tt>(in a Y)</tt>, then <tt>(subset X Y)</tt> is just</p>
+
+<code>
+ (forall a, (implies (in a X) (P a)))
+</code>
+
+<p>Our generalization basically lets you reduce a proof of <tt>(P-setp X)</tt>
+to a proof of <tt>(implies (in a X) (P a))</tt>, for an arbitrary predicate
+<tt>P</tt>.  This can be used to prove subset by just chooisng <tt>P</tt> as
+described above, but it can also be used for many other ideas by just changing
+the meaning of <tt>P</tt>.  For instance, if <tt>P</tt> is @(see integerp),
+then we can show that <tt>X</tt> is an <tt>integer-setp</tt> or similar.</p>
+
+<p>The mechanism is just an adaptation of that described in the previous
+section.</p>
+
+<ul>
+
+<li>We begin by introducing a completely arbitrary <tt>predicate</tt>.</li>
+
+<li>Based on <tt>predicate</tt>, we introduce a new function, <tt>all</tt>,
+which checks to see if every member in a set satisfies <tt>predicate</tt>.</li>
+
+<li>We set up an encapsulate which allows us to assume that some hypotheses are
+true and that any member of some set satisfies <tt>predicate</tt>.</li>
+
+</ul>
+
+<p>Finally, we prove <tt>all-by-membership</tt>, which shows that under these
+assumptions, the set satisfies <tt>all</tt>.  This theorem can be functionally
+instantiated to reduce a proof of <tt>(all X)</tt> to a proof of</p>
+
+<code>
+  (implies (in a X) (P a))
+</code>"
+
+  (encapsulate
+    (((predicate *) => *))
+    (local (defun predicate (x) x)))
+
+  (defun all (set-for-all-reduction)
+    (declare (xargs :guard (setp set-for-all-reduction)))
+    (if (empty set-for-all-reduction)
+        t
+      (and (predicate (head set-for-all-reduction))
+           (all (tail set-for-all-reduction)))))
+
+  (encapsulate
+    (((all-hyps) => *)
+     ((all-set) => *))
+
+    (local (defun all-hyps () nil))
+    (local (defun all-set () nil))
+
+    (defthmd membership-constraint
+      (implies (all-hyps)
+               (implies (in arbitrary-element (all-set))
+                        (predicate arbitrary-element)))))
+
+  (local (defun find-not (X)
+           (declare (xargs :guard (setp X)))
+           (cond ((empty X) nil)
+                 ((not (predicate (head X))) (head X))
+                 (t (find-not (tail X))))))
 
   (local (defthm lemma-find-not-is-a-witness
-	   (implies (not (all x))
-		    (and (in (find-not x) x)
-			 (not (predicate (find-not x)))))))
+           (implies (not (all x))
+                    (and (in (find-not x) x)
+                         (not (predicate (find-not x)))))))
 
   (defthmd all-by-membership
     (implies (all-hyps)
-	     (all (all-set)))
+             (all (all-set)))
     :hints(("Goal"
-	    :use (:instance membership-constraint
-			    (arbitrary-element (find-not (all-set))))))))
-
-
-; The theorem all-by-membership is massively important.  It is the basis for
-; reducing subset arguments to membership arguments.  It also has a
-; sufficiently general character that we can reuse it to make similar
-; reductions for problems other than subset.
-;
-; However, for the time being, it's important that we actually do apply this
-; theorem to the subset function, which is a particularly useful way of
-; reasoning about sets.  Two important questions are: how can we apply the
-; theorem, and when should we apply it?
-;
-; To support these notions, a framework is introduced in the file
-; computed-hints.lisp.  Basically, we introduce a "trigger" function which is
-; nothing more than an alias for subset.  We then use the "tagging theorem"
-; pick-a-point-subset-strategy in order to rewrite subsets into
-; subset-triggers.  This theorem is constrained so that it will only rewrite
-; conclusions and it will not apply while backchaining, via syntaxp hypotheses.
-; This process is described in more detail in computed-hints.lisp.
-
-(defun subset-trigger (X Y)
-  (declare (xargs :guard (and (setp X) (setp Y))))
-  (subset X Y))
-
-(defthm pick-a-point-subset-strategy
-  (implies (and (syntaxp (rewriting-goal-lit mfc state))
-		(syntaxp (rewriting-conc-lit `(subset ,X ,Y) mfc state)))
-	   (equal (subset X Y)
-		  (subset-trigger X Y))))
-
-(in-theory (disable subset-trigger))
-
-
-; BOZO replace all this stuff with witness-cp
-(COMPUTED-HINTS::automate-instantiation
-  :new-hint-name pick-a-point-subset-hint
-  :generic-theorem all-by-membership
-  :generic-predicate predicate
-  :generic-hyps all-hyps
-  :generic-collection all-set
-  :generic-collection-predicate all
-  :actual-collection-predicate subset
-  :actual-trigger subset-trigger
-  :predicate-rewrite (((predicate ?x ?y) (in ?x ?y)))
-  :tagging-theorem pick-a-point-subset-strategy)
+            :use (:instance membership-constraint
+                            (arbitrary-element (find-not (all-set))))))))
 
 
 
+(defsection pick-a-point-subset-strategy
+  :parents (osets)
+  :short "Automatic pick-a-point proofs of @(see subset)."
+
+  :long "<p>The rewrite rule <tt>pick-a-point-subset-strategy</tt> tries to
+automatically reduce proof goals such as:</p>
+
+<code>
+ (implies hyps
+          (subset X Y))
+</code>
+
+<p>To proofs of:</p>
+
+<code>
+ (implies (and hyps (in a X))
+          (in a Y))
+</code>
+
+<p>The mechanism for doing this is somewhat elaborate: the rewrite rule
+replaces the <tt>(subset X Y)</tt> with <tt>(subset-trigger X Y)</tt>.  This
+trigger is recognized by a computed hint, which then suggest proving the
+theorem via functional instantiation of @(see all-by-membership).</p>
+
+<p>The pick-a-point method is often a good way to prove subset relations.  On
+the other hand, this rule is very heavy-handed, and you may need to disable it
+if you do not want to use the pick-a-point method to solve your goal.</p>"
+
+  (defun subset-trigger (X Y)
+    (declare (xargs :guard (and (setp X) (setp Y))))
+    (subset X Y))
+
+  (defthm pick-a-point-subset-strategy
+    (implies (and (syntaxp (rewriting-goal-lit mfc state))
+                  (syntaxp (rewriting-conc-lit `(subset ,X ,Y) mfc state)))
+             (equal (subset X Y)
+                    (subset-trigger X Y))))
+
+  (in-theory (disable subset-trigger))
+
+  ;; BOZO replace all this stuff with witness-cp?
+  (COMPUTED-HINTS::automate-instantiation
+   :new-hint-name pick-a-point-subset-hint
+   :generic-theorem all-by-membership
+   :generic-predicate predicate
+   :generic-hyps all-hyps
+   :generic-collection all-set
+   :generic-collection-predicate all
+   :actual-collection-predicate subset
+   :actual-trigger subset-trigger
+   :predicate-rewrite (((predicate ?x ?y) (in ?x ?y)))
+   :tagging-theorem pick-a-point-subset-strategy))
 
 
-; We now show the basic properties of subset.  The first theorems are mundane
-; but then we get more interesting, showing that subset is reflexive and
-; transitive.  The goal here is to build up sufficient theorems to do
-; pick-a-point proofs, which come next.
 
-(defthm subset-sfix-cancel-X
-  (equal (subset (sfix X) Y)
-	 (subset X Y)))
 
-(defthm subset-sfix-cancel-Y
-  (equal (subset X (sfix Y))
-	 (subset X Y)))
+(defsection subset-theorems
+  :extension subset
 
-(defthm empty-subset
-  (implies (empty X)
-	   (subset X Y)))
+  (defthm subset-sfix-cancel-X
+    (equal (subset (sfix X) Y)
+           (subset X Y)))
 
-(defthm empty-subset-2
-  (implies (empty Y)
-	   (equal (subset X Y)
-                  (empty X))))
+  (defthm subset-sfix-cancel-Y
+    (equal (subset X (sfix Y))
+           (subset X Y)))
 
-(defthm subset-in
-  (and (implies (and (subset X Y)
-                     (in a X))
-                (in a Y))
-       (implies (and (in a X)
-                     (subset X Y))
-                (in a Y))))
+  (defthm empty-subset
+    (implies (empty X)
+             (subset X Y)))
 
-(defthm subset-in-2
-  (and (implies (and (subset X Y)
-                     (not (in a Y)))
-                (not (in a X)))
-       (implies (and (not (in a Y))
-                     (subset X Y))
-                (not (in a X)))))
+  (defthm empty-subset-2
+    (implies (empty Y)
+             (equal (subset X Y)
+                    (empty X))))
 
-(encapsulate
-  ()
-  (local (defthm l0
-           (equal (subset (insert a nil) Y)
+  (defthm subset-in
+    (and (implies (and (subset X Y)
+                       (in a X))
                   (in a Y))
-           :hints(("Goal" :in-theory (enable (:ruleset primitive-rules))))))
+         (implies (and (in a X)
+                       (subset X Y))
+                  (in a Y))))
 
-  (defthm subset-insert-X
-    (equal (subset (insert a X) Y)
-           (and (subset X Y)
-                (in a Y)))
-    :hints(("Goal" :induct (insert a X)))))
+  (defthm subset-in-2
+    (and (implies (and (subset X Y)
+                       (not (in a Y)))
+                  (not (in a X)))
+         (implies (and (not (in a Y))
+                       (subset X Y))
+                  (not (in a X)))))
 
-(defthm subset-reflexive
-  (subset X X))
+  (encapsulate
+    ()
+    (local (defthm l0
+             (equal (subset (insert a nil) Y)
+                    (in a Y))
+             :hints(("Goal" :in-theory (enable (:ruleset primitive-rules))))))
 
-(defthm subset-transitive
-  (implies (and (subset X Y)
-		(subset Y Z))
-           (subset X Z)))
+    (defthm subset-insert-X
+      (equal (subset (insert a X) Y)
+             (and (subset X Y)
+                  (in a Y)))
+      :hints(("Goal" :induct (insert a X)))))
 
-(defthm subset-membership-tail
-  (implies (and (subset X Y)
-		(in a (tail X)))
-           (in a (tail Y)))
-  :hints(("Goal" :in-theory (enable (:ruleset order-rules)))))
+  (defthm subset-reflexive
+    (subset X X))
 
-(defthm subset-membership-tail-2
-  (implies (and (subset X Y)
-		(not (in a (tail Y))))
-           (not (in a (tail X))))
-  :hints(("Goal" :in-theory (disable subset-membership-tail)
-                 :use (:instance subset-membership-tail))))
+  (defthm subset-transitive
+    (and (implies (and (subset X Y)
+                       (subset Y Z))
+                  (subset X Z))
+         (implies (and (subset Y Z)
+                       (subset X Y))
+                  (subset X Z))))
 
-(defthm subset-insert
-  (subset X (insert a X)))
+  (defthm subset-membership-tail
+    (implies (and (subset X Y)
+                  (in a (tail X)))
+             (in a (tail Y)))
+    :hints(("Goal" :in-theory (enable (:ruleset order-rules)))))
 
-(defthm subset-tail
-  (subset (tail X) X)
-  :rule-classes ((:rewrite)
-		 (:forward-chaining :trigger-terms ((tail x)))))
+  (defthm subset-membership-tail-2
+    (implies (and (subset X Y)
+                  (not (in a (tail Y))))
+             (not (in a (tail X))))
+    :hints(("Goal" :in-theory (disable subset-membership-tail)
+            :use (:instance subset-membership-tail))))
+
+  (defthm subset-insert
+    (subset X (insert a X)))
+
+  (defthm subset-tail
+    (subset (tail X) X)
+    :rule-classes ((:rewrite)
+                   (:forward-chaining :trigger-terms ((tail x))))))
 
 
 
 
+(defsection double-containment
+  :parents (osets)
+  :short "A strategy for proving sets are equal because they are subsets
+of one another."
 
+  :long "<p>Double containment can be a good way to prove that two sets are
+equal to one another.</p>
 
-; Proofs of equality by double containment are also very common.  So, to
-; support these, we want to show that double containment is the same as
-; equality.
-;
+<p>Unfortunately, because this rule targets <tt>equal</tt> it can get quite
+expensive.  You may sometimes wish to disable it to speed up your proofs, as
+directed by @(see accumulated-persistence).</p>"
+
 ; The general argument is the following:
 ;
 ; Suppose that we have two sets which are subsets of one another, i.e. (subset
@@ -594,8 +725,6 @@
 ; (tail X) = (tail Y).  Now, (head X) = (head Y) and (tail X) = (tail Y) can be
 ; used together to show that X = Y (see primitives.lisp, head-tail-same) so we
 ; are done.
-
-(encapsulate ()
 
 ; Here are the details.  First we show that the heads are the same:
 
@@ -677,10 +806,8 @@
     :hints(("Goal" :use (:instance double-containment-is-equality)))))
 
 
-; We are now done with the membership level.  We disable all of the
-; order based reasoning that we introduced here.
-
-; BOZO if we switch to rulesets we could add these to the primitives theory.
+; We are now done with the membership level.  We disable all of the order based
+; reasoning that we introduced here.
 
 (in-theory (disable head-minimal head-minimal-2))
 
