books/misc/total-order.lisp
@@ -3,31 +3,329 @@
 ; Sumners.
 
 (in-package "ACL2")
+(include-book "xdoc/top" :dir :system)
 
-(defun << (x y)
-  (declare (xargs :guard t))
-  (and (lexorder x y)
-       (not (equal x y))))
+; Jared added the definitions of fast-lexorder and fast-<< in order to speed up
+; ordered sets stuff.
 
-(defthm <<-irreflexive
-  (not (<< x x)))
+(defsection fast-lexorder
+  :parents (lexorder)
+  :short "Probably faster alternative to @(see lexorder)."
 
-(defthm <<-transitive
-  (implies (and (<< x y)
-                (<< y z))
-           (<< x z)))
+  :long "<p>@(call fast-lexorder) is logically the same as ACL2's built-in
+@(call lexorder), but is probably usually faster on real set elements.</p>
 
-(defthm <<-asymmetric
-  (implies (<< x y)
-           (not (<< y x))))
+<p>Conjecture: most \"real\" ACL2 objects are mainly built up from integers,
+symbols, and strings.  That is, non-integer numbers and characters are probably
+somewhat rare.</p>
 
-(defthm <<-trichotomy
-  (implies (and (not (<< y x))
-                (not (equal x y)))
-           (<< x y)))
+<p>ACL2's built-in <tt>lexorder</tt> uses @(see alphorder) to compare atoms.
+But <tt>alphorder</tt> first checks whether the elements are real or complex
+numbers, then characters, then finally strings or symbols.  This order isn't
+great if the conjecture above is true.  It seems especially unfortunate since
+<tt>real/rationalp</tt> and <tt>complex/complex-rationalp</tt> checks seem to
+be relatively expensive.  For instance, in CCL the following loop:</p>
 
-(defthm <<-implies-lexorder
-  (implies (<< x y)
-	   (lexorder x y)))
+<code>
+ (loop for a in
+   '(\"foo\" 3 #\a 'foo (expt 2 80) 1/3 (complex 3 4))
+    do (format t \"---- ~a ------~%\" a)
+       (time (loop for i fixnum from 1 to 1000000000
+                do (stringp a)))
+       (time (loop for i fixnum from 1 to 1000000000
+                do (integerp a)))
+       (time (loop for i fixnum from 1 to 1000000000
+                do (symbolp a)))
+       (time (loop for i fixnum from 1 to 1000000000
+                do (characterp a)))
+       (time (loop for i fixnum from 1 to 1000000000
+                do (real/rationalp a)))
+       (time (loop for i fixnum from 1 to 1000000000
+                 do (complex/complex-rationalp a))))
+</code>
 
-(in-theory (disable <<))
+<p>Appears to indicate that:</p>
+
+<ul>
+ <li><tt>characterp</tt> is the very fastest (~.7 seconds)</li>
+ <li><tt>symbolp</tt> is the next fastest (~1 second)</li>
+ <li><tt>integerp</tt> and <tt>stringp</tt> are the next fastest (~1.6 seconds)</li>
+ <li><tt>complex/complex-rationalp</tt> is slower (~3.6 seconds)</li>
+ <li><tt>real/rationalp</tt> is much slower (4-6 seconds seconds)</li>
+</ul>
+
+<p>The <tt>fast-lexorder</tt> function just rearranges things so that we first
+check for integers, strings, and symbols, which optimizes for our expected data
+distribution and avoids these expensive checks.  It also inlines this
+rearranged <tt>alphorder</tt> check into the top-level function to avoid the
+overhead of calling another function for each atom comparison.</p>
+
+<p>This seems to give us a nice speedup:</p>
+
+<code>
+ (loop for elem in
+   '( (1 . 2)                                  ;  1.238 vs 0.835
+      (\"foo\" . \"bar\")                          ;  6.525 vs 4.833
+      (foo . bar)                              ;  8.044 vs 5.860
+      (foo . foo)                              ; 19.895 vs 0.983 !
+      (#\\a . #\\b)                              ;  2.548 vs 1.140
+      ((\"foo\" . 1) . (\"bar\" . 1))              ;  9.661 vs 7.903
+      ((:foo \"foo\" . 1) . (:foo \"bar\" . 1)))   ; 10.064 vs 8.456
+   do
+   (let ((a (car elem))
+         (b (cdr elem)))
+     (format t \"---- ~a vs. ~a ------~%\" a b)
+     (time (loop for i fixnum from 1 to 100000000
+              do (lexorder a b)))
+     (time (loop for i fixnum from 1 to 100000000
+              do (fast-lexorder a b)))))
+</code>"
+
+  (defund fast-lexorder (x y)
+    (declare (xargs :guard t))
+    (cond ((atom x)
+           (if (atom y)
+
+               ;; Inlined, rearranged alphorder.
+               (cond ((integerp x)
+                      (cond ((integerp y)
+                             (<= x y))
+                            ((real/rationalp y)
+                             (<= x y))
+                            (t
+                             t)))
+
+                     ((symbolp x)
+                      (if (symbolp y)
+                          ;; Doing an EQ check here costs relatively very
+                          ;; little.  After all, we're about to do a function
+                          ;; call and two string compares.  And if it hits,
+                          ;; it's a big win.
+                          (or (eq x y)
+                              (and (symbol-< x y) t))
+                        ;; Ugh.  We should just know this is true, but we have
+                        ;; to consider these cases because of bad atoms:
+                        (not (or (integerp y)
+                                 (stringp y)
+                                 (characterp y)
+                                 (real/rationalp y)
+                                 (complex/complex-rationalp y)))))
+
+                     ((stringp x)
+                      (cond ((stringp y)
+                             (and (string<= x y) t))
+                            ((integerp y)
+                             nil)
+                            ((symbolp y)
+                             t)
+                            (t
+                             (not (or (characterp y)
+                                      (real/rationalp y)
+                                      (complex/complex-rationalp y))))))
+
+                     ((characterp x)
+                      (cond ((characterp y)
+                             (<= (char-code x) (char-code y)))
+                            (t
+                             (not (or (integerp y)
+                                      (real/rationalp y)
+                                      (complex/complex-rationalp y))))))
+
+                     ((real/rationalp x)
+                      (cond ((integerp y)
+                             (<= x y))
+                            ((real/rationalp y)
+                             (<= x y))
+                            (t t)))
+
+                     ((real/rationalp y)
+                      nil)
+
+                     ((complex/complex-rationalp x)
+                      (cond ((complex/complex-rationalp y)
+                             (or (< (realpart x)
+                                    (realpart y))
+                                 (and (= (realpart x)
+                                         (realpart y))
+                                      (<= (imagpart x)
+                                          (imagpart y)))))
+                            (t t)))
+
+                     ;; Ugly, just need this in case of bad-atoms.
+                     ((or (symbolp y)
+                          (stringp y)
+                          (characterp y)
+                          (complex/complex-rationalp y))
+                      nil)
+
+                     (t
+                      (acl2::bad-atom<= x y)))
+
+             ;; (atom x) and not (atom y)
+             t))
+          ((atom y)
+           nil)
+          ((equal (car x) (car y))
+           (fast-lexorder (cdr x) (cdr y)))
+          (t
+           (fast-lexorder (car x) (car y)))))
+
+  (local (in-theory (enable fast-lexorder lexorder alphorder)))
+
+  (defthm fast-lexorder-is-lexorder
+    (equal (fast-lexorder x y)
+           (lexorder x y))))
+
+
+(defsection fast-<<
+  :parents (<<)
+  :short "Probably faster alternative to @(see <<)."
+
+  :long "<p>@(call fast-<<) is logically the same as @(call <<).  However, it
+is probably faster because:</p>
+
+<ol>
+ <li>it rearranges the check as in @(see fast-lexorder), and</li>
+ <li>it folds in the not-equal check.</li>
+</ol>"
+
+  (defund fast-<< (x y)
+    (declare (xargs :guard t))
+    (cond ((atom x)
+           (if (atom y)
+               (cond ((integerp x)
+                      (cond ((integerp y)
+                             (< x y))
+                            ((real/rationalp y)
+                             (< x y))
+                            (t
+                             t)))
+                     ((symbolp x)
+                      (if (symbolp y)
+                          (and (not (eq x y))
+                               (symbol-< x y)
+                               t)
+                        (not (or (integerp y)
+                                 (stringp y)
+                                 (characterp y)
+                                 (real/rationalp y)
+                                 (complex/complex-rationalp y)))))
+                     ((stringp x)
+                      (cond ((stringp y)
+                             (and (string< x y) t))
+                            ((integerp y)
+                             nil)
+                            ((symbolp y)
+                             t)
+                            (t
+                             (not (or (characterp y)
+                                      (real/rationalp y)
+                                      (complex/complex-rationalp y))))))
+                     ((characterp x)
+                      (cond ((characterp y)
+                             (< (char-code x) (char-code y)))
+                            (t
+                             (not (or (integerp y)
+                                      (real/rationalp y)
+                                      (complex/complex-rationalp y))))))
+                     ((real/rationalp x)
+                      (cond ((integerp y)
+                             (< x y))
+                            ((real/rationalp y)
+                             (< x y))
+                            (t t)))
+                     ((real/rationalp y)
+                      nil)
+                     ((complex/complex-rationalp x)
+                      (cond ((complex/complex-rationalp y)
+                             (or (< (realpart x)
+                                    (realpart y))
+                                 (and (= (realpart x)
+                                         (realpart y))
+                                      (< (imagpart x)
+                                         (imagpart y)))))
+                            (t t)))
+                     ((or (symbolp y)
+                          (stringp y)
+                          (characterp y)
+                          (complex/complex-rationalp y))
+                      nil)
+                     (t
+                      (and (acl2::bad-atom<= x y)
+                           (not (equal x y)))))
+             t))
+          ((atom y)
+           nil)
+          ((equal (car x) (car y))
+           (fast-<< (cdr x) (cdr y)))
+          (t
+           (fast-<< (car x) (car y))))))
+
+
+(defsection <<
+  :parents (programming)
+  :short "A total ordering on ACL2 objects."
+
+  :long "<p>@(call <<) is a total ordering on ACL2 objects, defined in the
+<tt>misc/total-order</tt> book.  For more information about the development of
+this order, see the associated workshop paper:</p>
+
+<p>Matt Kaufmann and Pete Manolios.  <i><a
+href='http://www.cs.utexas.edu/users/moore/acl2/workshop-2002/contrib/manolios-kaufmann/total-order.pdf'>Adding
+a Total Order to ACL2</a>.</i> ACL2 Workshop, 2002.</p>
+
+<p>Efficiency note.  In the implementation, we generally use @(see fast-<<) and
+@(see fast-lexorder), which are probably faster alternatives to
+<tt>&lt;&lt;</tt> and <tt>lexorder</tt>, respectively.</p>"
+
+  (defund << (x y)
+    (declare (xargs :guard t
+                    :verify-guards nil))
+    (mbe :logic
+         (and (lexorder x y)
+              (not (equal x y)))
+         :exec
+         (fast-<< x y)))
+
+  (local (in-theory (enable <<)))
+
+  (defthm <<-irreflexive
+    (not (<< x x)))
+
+  (defthm <<-transitive
+    (implies (and (<< x y)
+                  (<< y z))
+             (<< x z)))
+
+  (defthm <<-asymmetric
+    (implies (<< x y)
+             (not (<< y x))))
+
+  (defthm <<-trichotomy
+    (implies (and (not (<< y x))
+                  (not (equal x y)))
+             (<< x y)))
+
+  (defthm <<-implies-lexorder
+    (implies (<< x y)
+             (lexorder x y))))
+
+
+(defsection fast-<<-correct
+  :extension fast-<<
+
+  (local (in-theory (enable fast-<< << lexorder alphorder)))
+
+  (local (defthm l0
+           (implies (and (characterp x)
+                         (characterp y))
+                    (equal (equal (char-code x) (char-code y))
+                           (equal x y)))
+           :hints(("Goal" :use ((:instance equal-char-code))))))
+
+  (defthm fast-<<-is-<<
+    (equal (fast-<< x y)
+           (<< x y))))
+
+(verify-guards <<
+  :hints(("Goal" :in-theory (enable <<))))
